make argument names more meaningful

code/sha2-mb/Hacl.SHA2.Scalar32.fst
@@ -22,94 +22,94 @@ module SpecVec = Hacl.Spec.SHA2.Vec
 [@CInline]
 private
 val sha224_update1: update_vec_t SHA2_224 M32
-let sha224_update1 b hash = update #SHA2_224 #M32 b hash
+let sha224_update1 block hash = update #SHA2_224 #M32 block hash
 
 
-val sha224: hash:lbuffer uint8 28ul -> len:size_t -> b:lbuffer uint8 len ->
+val sha224: dst:lbuffer uint8 28ul -> input_len:size_t -> input:lbuffer uint8 input_len ->
   Stack unit
-  (requires fun h0 -> v len <= max_input_length SHA2_224 /\
-    live h0 b /\ live h0 hash /\ disjoint hash b)
-  (ensures  fun h0 _ h1 -> modifies (loc hash) h0 h1 /\
-    as_seq h1 hash == Spec.hash SHA2_224 (as_seq h0 b))
+  (requires fun h0 -> v input_len <= max_input_length SHA2_224 /\
+    live h0 input /\ live h0 dst /\ disjoint dst input)
+  (ensures  fun h0 _ h1 -> modifies (loc dst) h0 h1 /\
+    as_seq h1 dst == Spec.hash SHA2_224 (as_seq h0 input))
 
-let sha224 h len b =
+let sha224 dst input_len input =
+  let ib = ntup1 input in
+  let rb = ntup1 dst in
   let h0 = ST.get() in
-  let b = ntup1 b in
-  let h = ntup1 h in
-  hash #SHA2_224 #M32 (sha224_update1 <: update_vec_t SHA2_224 M32) h len b;
+  loc_multi1 rb;
+  hash #SHA2_224 #M32 (sha224_update1 <: update_vec_t SHA2_224 M32) rb input_len ib;
   let h1 = ST.get() in
-  Hacl.Spec.SHA2.Equiv.hash_agile_lemma #SHA2_224 #M32 (v len) (as_seq_multi h0 b);
-  let hash0 = tup1 h in
-  assert ((as_seq_multi h1 h).(|0|) == as_seq h1 hash0)
+  Hacl.Spec.SHA2.Equiv.hash_agile_lemma #SHA2_224 #M32 (v input_len) (as_seq_multi h0 ib);
+  assert ((as_seq_multi h1 rb).(|0|) == as_seq h1 dst)
 
 
 [@CInline]
 private
 val sha256_update1: update_vec_t SHA2_256 M32
-let sha256_update1 b hash = update #SHA2_256 #M32 b hash
+let sha256_update1 block hash = update #SHA2_256 #M32 block hash
 
 
-val sha256: hash:lbuffer uint8 32ul -> len:size_t -> b:lbuffer uint8 len ->
+val sha256: dst:lbuffer uint8 32ul -> input_len:size_t -> input:lbuffer uint8 input_len ->
   Stack unit
-  (requires fun h0 -> v len <= max_input_length SHA2_256 /\
-    live h0 b /\ live h0 hash /\ disjoint hash b)
-  (ensures  fun h0 _ h1 -> modifies (loc hash) h0 h1 /\
-    as_seq h1 hash == Spec.hash SHA2_256 (as_seq h0 b))
+  (requires fun h0 -> v input_len <= max_input_length SHA2_256 /\
+    live h0 input /\ live h0 dst /\ disjoint dst input)
+  (ensures  fun h0 _ h1 -> modifies (loc dst) h0 h1 /\
+    as_seq h1 dst == Spec.hash SHA2_256 (as_seq h0 input))
 
-let sha256 h len b =
+let sha256 dst input_len input =
+  let ib = ntup1 input in
+  let rb = ntup1 dst in
   let h0 = ST.get() in
-  let b = ntup1 b in
-  let h = ntup1 h in
-  hash #SHA2_256 #M32 (sha256_update1 <: update_vec_t SHA2_256 M32) h len b;
+  loc_multi1 rb;
+  hash #SHA2_256 #M32 (sha256_update1 <: update_vec_t SHA2_256 M32) rb input_len ib;
   let h1 = ST.get() in
-  Hacl.Spec.SHA2.Equiv.hash_agile_lemma #SHA2_256 #M32 (v len) (as_seq_multi h0 b);
-  let hash0 = tup1 h in
-  assert ((as_seq_multi h1 h).(|0|) == as_seq h1 hash0)
+  Hacl.Spec.SHA2.Equiv.hash_agile_lemma #SHA2_256 #M32 (v input_len) (as_seq_multi h0 ib);
+  assert ((as_seq_multi h1 rb).(|0|) == as_seq h1 dst)
 
 
 [@CInline]
 private
 val sha384_update1: update_vec_t SHA2_384 M32
-let sha384_update1 b hash = update #SHA2_384 #M32 b hash
+let sha384_update1 block hash = update #SHA2_384 #M32 block hash
 
 
-val sha384: hash:lbuffer uint8 48ul -> len:size_t -> b:lbuffer uint8 len ->
+val sha384: dst:lbuffer uint8 48ul -> input_len:size_t -> input:lbuffer uint8 input_len ->
   Stack unit
-  (requires fun h0 ->  v len <= max_input_length SHA2_384 /\
-    live h0 b /\ live h0 hash /\ disjoint hash b)
-  (ensures  fun h0 _ h1 -> modifies (loc hash) h0 h1 /\
-    as_seq h1 hash == Spec.hash SHA2_384 (as_seq h0 b))
+  (requires fun h0 -> v input_len <= max_input_length SHA2_384 /\
+    live h0 input /\ live h0 dst /\ disjoint dst input)
+  (ensures  fun h0 _ h1 -> modifies (loc dst) h0 h1 /\
+    as_seq h1 dst == Spec.hash SHA2_384 (as_seq h0 input))
 
-let sha384 h len b =
+let sha384 dst input_len input =
+  let ib = ntup1 input in
+  let rb = ntup1 dst in
   let h0 = ST.get() in
-  let b = ntup1 b in
-  let h = ntup1 h in
-  hash #SHA2_384 #M32 (sha384_update1 <: update_vec_t SHA2_384 M32) h len b;
+  loc_multi1 rb;
+  hash #SHA2_384 #M32 (sha384_update1 <: update_vec_t SHA2_384 M32) rb input_len ib;
   let h1 = ST.get() in
-  Hacl.Spec.SHA2.Equiv.hash_agile_lemma #SHA2_384 #M32 (v len) (as_seq_multi h0 b);
-  let hash0 = tup1 h in
-  assert ((as_seq_multi h1 h).(|0|) == as_seq h1 hash0)
+  Hacl.Spec.SHA2.Equiv.hash_agile_lemma #SHA2_384 #M32 (v input_len) (as_seq_multi h0 ib);
+  assert ((as_seq_multi h1 rb).(|0|) == as_seq h1 dst)
 
 
 [@CInline]
 private
 val sha512_update1: update_vec_t SHA2_512 M32
-let sha512_update1 b hash = update #SHA2_512 #M32 b hash
+let sha512_update1 block hash = update #SHA2_512 #M32 block hash
 
 
-val sha512: hash:lbuffer uint8 64ul -> len:size_t -> b:lbuffer uint8 len ->
+val sha512: dst:lbuffer uint8 64ul -> input_len:size_t -> input:lbuffer uint8 input_len ->
   Stack unit
-  (requires fun h0 -> v len <= max_input_length SHA2_512 /\
-    live h0 b /\ live h0 hash /\ disjoint hash b)
-  (ensures  fun h0 _ h1 -> modifies (loc hash) h0 h1 /\
-    as_seq h1 hash == Spec.hash SHA2_512 (as_seq h0 b))
+  (requires fun h0 -> v input_len <= max_input_length SHA2_512 /\
+    live h0 input /\ live h0 dst /\ disjoint dst input)
+  (ensures  fun h0 _ h1 -> modifies (loc dst) h0 h1 /\
+    as_seq h1 dst == Spec.hash SHA2_512 (as_seq h0 input))
 
-let sha512 h len b =
+let sha512 dst input_len input =
+  let ib = ntup1 input in
+  let rb = ntup1 dst in
   let h0 = ST.get() in
-  let b = ntup1 b in
-  let h = ntup1 h in
-  hash #SHA2_512 #M32 (sha512_update1 <: update_vec_t SHA2_512 M32) h len b;
+  loc_multi1 rb;
+  hash #SHA2_512 #M32 (sha512_update1 <: update_vec_t SHA2_512 M32) rb input_len ib;
   let h1 = ST.get() in
-  Hacl.Spec.SHA2.Equiv.hash_agile_lemma #SHA2_512 #M32 (v len) (as_seq_multi h0 b);
-  let hash0 = tup1 h in
-  assert ((as_seq_multi h1 h).(|0|) == as_seq h1 hash0)
+  Hacl.Spec.SHA2.Equiv.hash_agile_lemma #SHA2_512 #M32 (v input_len) (as_seq_multi h0 ib);
+  assert ((as_seq_multi h1 rb).(|0|) == as_seq h1 dst)
