code/sha2-mb/Hacl.SHA2.Vec128.fst
@@ -23,66 +23,68 @@ module SpecVec = Hacl.Spec.SHA2.Vec
 [@CInline]
 private
 val sha224_update4: update_vec_t SHA2_224 M128
-let sha224_update4 b hash = update #SHA2_224 #M128 b hash
+let sha224_update4 block hash = update #SHA2_224 #M128 block hash
 
 
-val sha224_4 (r0 r1 r2 r3: lbuffer uint8 28ul) (len:size_t) (b0 b1 b2 b3: lbuffer uint8 len) :
+val sha224_4 (dst0 dst1 dst2 dst3: lbuffer uint8 28ul) (input_len:size_t) (input0 input1 input2 input3: lbuffer uint8 input_len) :
   Stack unit
-  (requires fun h0 -> v len <= max_input_length SHA2_224 /\
-    live4 h0 b0 b1 b2 b3 /\ live4 h0 r0 r1 r2 r3 /\ internally_disjoint4 r0 r1 r2 r3)
-  (ensures  fun h0 _ h1 -> modifies (loc r0 |+| loc r1 |+| loc r2 |+| loc r3) h0 h1 /\
-    as_seq h1 r0 == Spec.hash SHA2_224 (as_seq h0 b0) /\
-    as_seq h1 r1 == Spec.hash SHA2_224 (as_seq h0 b1) /\
-    as_seq h1 r2 == Spec.hash SHA2_224 (as_seq h0 b2) /\
-    as_seq h1 r3 == Spec.hash SHA2_224 (as_seq h0 b3))
+  (requires fun h0 -> v input_len <= max_input_length SHA2_224 /\
+    live4 h0 input0 input1 input2 input3 /\
+    live4 h0 dst0 dst1 dst2 dst3 /\
+    internally_disjoint4 dst0 dst1 dst2 dst3)
+  (ensures  fun h0 _ h1 -> modifies (loc dst0 |+| loc dst1 |+| loc dst2 |+| loc dst3) h0 h1 /\
+    as_seq h1 dst0 == Spec.hash SHA2_224 (as_seq h0 input0) /\
+    as_seq h1 dst1 == Spec.hash SHA2_224 (as_seq h0 input1) /\
+    as_seq h1 dst2 == Spec.hash SHA2_224 (as_seq h0 input2) /\
+    as_seq h1 dst3 == Spec.hash SHA2_224 (as_seq h0 input3))
 
-let sha224_4 r0 r1 r2 r3 len b0 b1 b2 b3 =
-  let h0 = ST.get() in
-  let ib = ntup4 (b0,(b1,(b2,b3))) in
-  let rb = ntup4 (r0,(r1,(r2,r3))) in
+let sha224_4 dst0 dst1 dst2 dst3 input_len input0 input1 input2 input3 =
+  let ib = ntup4 (input0,(input1,(input2,input3))) in
+  let rb = ntup4 (dst0,(dst1,(dst2,dst3))) in
   let h0 = ST.get() in
   assert (live_multi h0 ib);
   assert (live_multi h0 rb);
   assert (internally_disjoint rb);
   loc_multi4 rb;
-  hash #SHA2_224 #M128 sha224_update4 rb len ib;
+  hash #SHA2_224 #M128 sha224_update4 rb input_len ib;
   let h1 = ST.get() in
-  Hacl.Spec.SHA2.Equiv.hash_agile_lemma #SHA2_224 #M128 (v len) (as_seq_multi h0 ib);
-  assert ((as_seq_multi h1 rb).(|0|) == as_seq h1 r0);
-  assert ((as_seq_multi h1 rb).(|1|) == as_seq h1 r1);
-  assert ((as_seq_multi h1 rb).(|2|) == as_seq h1 r2);
-  assert ((as_seq_multi h1 rb).(|3|) == as_seq h1 r3)
+  Hacl.Spec.SHA2.Equiv.hash_agile_lemma #SHA2_224 #M128 (v input_len) (as_seq_multi h0 ib);
+  assert ((as_seq_multi h1 rb).(|0|) == as_seq h1 dst0);
+  assert ((as_seq_multi h1 rb).(|1|) == as_seq h1 dst1);
+  assert ((as_seq_multi h1 rb).(|2|) == as_seq h1 dst2);
+  assert ((as_seq_multi h1 rb).(|3|) == as_seq h1 dst3)
 
 
 [@CInline]
 private
 val sha256_update4: update_vec_t SHA2_256 M128
-let sha256_update4 b hash = update #SHA2_256 #M128 b hash
+let sha256_update4 block hash = update #SHA2_256 #M128 block hash
 
 
-val sha256_4 (r0 r1 r2 r3: lbuffer uint8 32ul) (len:size_t) (b0 b1 b2 b3: lbuffer uint8 len) :
+val sha256_4 (dst0 dst1 dst2 dst3: lbuffer uint8 32ul) (input_len:size_t) (input0 input1 input2 input3: lbuffer uint8 input_len) :
   Stack unit
-  (requires fun h0 -> v len <= max_input_length SHA2_256 /\
-    live4 h0 b0 b1 b2 b3 /\ live4 h0 r0 r1 r2 r3 /\ internally_disjoint4 r0 r1 r2 r3)
-  (ensures  fun h0 _ h1 -> modifies (loc r0 |+| loc r1 |+| loc r2 |+| loc r3) h0 h1 /\
-    as_seq h1 r0 == Spec.hash SHA2_256 (as_seq h0 b0) /\
-    as_seq h1 r1 == Spec.hash SHA2_256 (as_seq h0 b1) /\
-    as_seq h1 r2 == Spec.hash SHA2_256 (as_seq h0 b2) /\
-    as_seq h1 r3 == Spec.hash SHA2_256 (as_seq h0 b3))
+  (requires fun h0 -> v input_len <= max_input_length SHA2_256 /\
+    live4 h0 input0 input1 input2 input3 /\
+    live4 h0 dst0 dst1 dst2 dst3 /\
+    internally_disjoint4 dst0 dst1 dst2 dst3)
+  (ensures  fun h0 _ h1 -> modifies (loc dst0 |+| loc dst1 |+| loc dst2 |+| loc dst3) h0 h1 /\
+    as_seq h1 dst0 == Spec.hash SHA2_256 (as_seq h0 input0) /\
+    as_seq h1 dst1 == Spec.hash SHA2_256 (as_seq h0 input1) /\
+    as_seq h1 dst2 == Spec.hash SHA2_256 (as_seq h0 input2) /\
+    as_seq h1 dst3 == Spec.hash SHA2_256 (as_seq h0 input3))
 
-let sha256_4 r0 r1 r2 r3 len b0 b1 b2 b3 =
-  let h0 = ST.get() in
-  let ib = ntup4 (b0,(b1,(b2,b3))) in
-  let rb = ntup4 (r0,(r1,(r2,r3))) in
+let sha256_4 dst0 dst1 dst2 dst3 input_len input0 input1 input2 input3 =
+  let ib = ntup4 (input0,(input1,(input2,input3))) in
+  let rb = ntup4 (dst0,(dst1,(dst2,dst3))) in
   let h0 = ST.get() in
   assert (live_multi h0 ib);
   assert (live_multi h0 rb);
   assert (internally_disjoint rb);
   loc_multi4 rb;
-  hash #SHA2_256 #M128 sha256_update4 rb len ib;
+  hash #SHA2_256 #M128 sha256_update4 rb input_len ib;
   let h1 = ST.get() in
-  Hacl.Spec.SHA2.Equiv.hash_agile_lemma #SHA2_256 #M128 (v len) (as_seq_multi h0 ib);
-  assert ((as_seq_multi h1 rb).(|0|) == as_seq h1 r0);
-  assert ((as_seq_multi h1 rb).(|1|) == as_seq h1 r1);
-  assert ((as_seq_multi h1 rb).(|2|) == as_seq h1 r2);
-  assert ((as_seq_multi h1 rb).(|3|) == as_seq h1 r3)
+  Hacl.Spec.SHA2.Equiv.hash_agile_lemma #SHA2_256 #M128 (v input_len) (as_seq_multi h0 ib);
+  assert ((as_seq_multi h1 rb).(|0|) == as_seq h1 dst0);
+  assert ((as_seq_multi h1 rb).(|1|) == as_seq h1 dst1);
+  assert ((as_seq_multi h1 rb).(|2|) == as_seq h1 dst2);
+  assert ((as_seq_multi h1 rb).(|3|) == as_seq h1 dst3)
